Switch everything to use higher-order saved predicates

theories/dlang.v
@@ -3,7 +3,7 @@ From iris.proofmode Require Import tactics.
 From iris.program_logic Require Import ectx_language language.
 
 From D.pure_program_logic Require adequacy.
-From D Require gen_iheap saved_interp.
+From D Require gen_iheap saved_interp_dep.
 
 Module mapsto.
 Export gen_iheap.
@@ -20,18 +20,20 @@ End mapsto_stamp_gname.
 End mapsto.
 
 Module Type LiftWp (Import VS : VlSortsSig).
-  Export mapsto saved_interp.
+  Export mapsto saved_interp_dep.
   Implicit Types (v : vl) (vs : vls) (Σ : gFunctors).
+  Include SavedInterpDep VS.
 
-  Notation envPred s Σ := ((var → vl) -d> s -d> iProp Σ).
+  Notation savedHoSemTypeG Σ := (savedHoEnvPredG vl Σ).
+  Notation savedHoSemTypeΣ := (savedHoEnvPredΣ vl).
+
   Instance InhEnvPred s Σ : Inhabited (envPred s Σ) := populate (λ _ _, False)%I.
-  Notation envD Σ := (envPred vl Σ).
 
   Class TyInterp ty Σ :=
-    ty_interp : ty -> (var → vl) -> vl -> iProp Σ.
+    ty_interp : ty -> envD Σ.
 
   Class dlangG Σ := DLangG {
-    dlangG_savior :> savedInterpG Σ (var → vl) vl;
+    dlangG_savior :> savedHoSemTypeG Σ;
     dlangG_interpNames :> gen_iheapG stamp gname Σ;
   }.
 
@@ -54,38 +56,71 @@ Module Type LiftWp (Import VS : VlSortsSig).
     iApply (wp_wand with "[-]"); [iApply Hp; trivial|]; cbn;
     iIntros (v) Hv.
 
-  Notation "s ↝ φ" := (∃ γ, s ↦ γ ∗ γ ⤇ φ)%I  (at level 20) : bi_scope.
+  Definition stamp_to_type_n `{!dlangG Σ}
+    s n (φ : hoEnvD Σ n) := (∃ γ, (s ↦ γ) ∗ γ ⤇n[ n ] φ)%I.
+  Notation "s ↝n[ n  ] φ" := (stamp_to_type_n s n φ) (at level 20) : bi_scope.
 
-  Definition stamp_σ_to_type `{!dlangG Σ} s σ (ψ : vl -d> iProp Σ) : iProp Σ :=
-    (∃ φ : envD Σ, ⌜ ψ = φ (to_subst σ) ⌝ ∗ s ↝ φ)%I.
-  Notation "s ↗[ σ  ] ψ" := (stamp_σ_to_type s σ ψ) (at level 20).
+  Definition hoEnvD_inst {n Σ} (φ : hoEnvD Σ n) σ : hoD Σ n := λ args, φ args (to_subst σ).
+
+  Definition stamp_σ_to_type_n `{!dlangG Σ} s σ n (ψ : hoD Σ n) : iProp Σ :=
+    (∃ φ : hoEnvD Σ n, ⌜ ψ = hoEnvD_inst φ σ ⌝ ∗ s ↝n[ n ] φ)%I.
+  Notation "s ↗n[ σ , n  ] ψ" := (stamp_σ_to_type_n s σ n ψ) (at level 20): bi_scope.
+
+  Notation "γ ⤇ φ" := (γ ⤇n[ 0 ] vopen φ) (at level 20).
+  Notation "s ↝ φ" := (s ↝n[ 0 ] vopen φ)%I  (at level 20) : bi_scope.
+  Notation "s ↗[ σ  ] ψ" := (s ↗n[ σ , 0 ] vopen ψ)%I (at level 20) : bi_scope.
 
   Section mapsto.
     Context `{!dlangG Σ}.
 
-    Global Instance stamp_σ_to_type_persistent σ s ψ: Persistent (s ↗[ σ  ] ψ) := _.
+    Global Instance: Persistent (s ↝n[ n ] φ) := _.
 
-    Lemma stamp_σ_to_type_agree σ s ψ1 ψ2 v :
-      s ↗[ σ ] ψ1 -∗ s ↗[ σ ] ψ2 -∗ ▷ (ψ1 v ≡ ψ2 v).
+    Global Instance stamp_σ_to_type_persistent σ s n ψ : Persistent (s ↗n[ σ , n ] ψ) := _.
+
+    Lemma stamp_σ_to_type_agree_dep_arity {σ s n1 n2 ψ1 ψ2} :
+      s ↗n[ σ , n1 ] ψ1 -∗ s ↗n[ σ , n2 ] ψ2 -∗ ⌜ n1 = n2 ⌝.
     Proof.
       iDestruct 1 as (φ1 -> γ1) "[Hs1 Hg1]".
       iDestruct 1 as (φ2 -> γ2) "[Hs2 Hg2]".
       iDestruct (mapsto_agree with "Hs1 Hs2") as %->.
-      iApply (saved_interp_agree with "Hg1 Hg2").
+      iDestruct (saved_ho_sem_type_agree_arity with "Hg1 Hg2") as %->.
+      by [].
     Qed.
 
-    Lemma stamp_σ_to_type_intro s σ φ : s ↝ φ -∗ s ↗[ σ ] φ (to_subst σ).
-    Proof. rewrite /stamp_σ_to_type. iIntros; iExists φ; auto. Qed.
+    Import EqNotations.
+    Lemma stamp_σ_to_type_agree_dep {σ s n1 n2 ψ1 ψ2} args v :
+      s ↗n[ σ , n1 ] ψ1 -∗ s ↗n[ σ , n2 ] ψ2 -∗ ∃ eq : n1 = n2,
+        ▷ ((rew [hoD Σ] eq in ψ1) args v ≡ ψ2 args v).
+    Proof.
+      iDestruct 1 as (φ1 -> γ1) "[Hs1 Hg1]".
+      iDestruct 1 as (φ2 -> γ2) "[Hs2 Hg2]".
+      iDestruct (mapsto_agree with "Hs1 Hs2") as %->.
+      iDestruct (saved_ho_sem_type_agree_arity with "Hg1 Hg2") as %->.
+      iExists eq_refl; cbn.
+      iApply (saved_ho_sem_type_agree with "Hg1 Hg2").
+    Qed.
+
+    Lemma stamp_σ_to_type_agree {σ s n ψ1 ψ2} args v :
+      s ↗n[ σ , n ] ψ1 -∗ s ↗n[ σ , n ] ψ2 -∗ ▷ (ψ1 args v ≡ ψ2 args v).
+    Proof.
+      iIntros "Hs1 Hs2".
+      iDestruct (stamp_σ_to_type_agree_dep args v with "Hs1 Hs2") as (eq) "H".
+      rewrite (proof_irrel eq eq_refl) /=. by [].
+    Qed.
+
+    Lemma stamp_σ_to_type_intro s σ n (φ : hoEnvD Σ n) :
+      s ↝n[ n ] φ -∗ s ↗n[ σ , n ] hoEnvD_inst φ σ.
+    Proof. rewrite /stamp_σ_to_type_n. iIntros; iExists φ; auto. Qed.
   End mapsto.
 
-  Global Opaque stamp_σ_to_type.
+  Global Opaque stamp_σ_to_type_n.
 
   Module dlang_adequacy.
     Class dlangPreG Σ := DLangPreG {
-      dlangPreG_savior :> savedInterpG Σ (var → vl) vl;
+      dlangPreG_savior :> savedHoSemTypeG Σ;
       dlangPreG_interpNames :> gen_iheapPreG stamp gname Σ;
     }.
-    Definition dlangΣ := #[savedInterpΣ (var → vl) vl; gen_iheapΣ stamp gname].
+    Definition dlangΣ := #[savedHoSemTypeΣ; gen_iheapΣ stamp gname].
 
     Instance subG_dlangΣ {Σ} : subG dlangΣ Σ → dlangPreG Σ.
     Proof. solve_inG. Qed.
